More work on automata

Cslib/Computability/Automata/Acceptor.lean
@@ -9,9 +9,9 @@ import Cslib.Computability.Languages.Language
 namespace Cslib.Automata
 
 /-- An `Acceptor` is a machine that recognises strings (lists of symbols in an alphabet). -/
-structure Acceptor (Symbol : Type _) where
+class Acceptor (α : Type _) (Symbol : outParam (Type _)) where
   /-- Predicate that establishes whether a string `xs` is accepted. -/
-  Accepts (xs : List Symbol) : Prop
+  Accepts (a : α) (xs : List Symbol) : Prop
 
 namespace Acceptor
 
@@ -19,13 +19,13 @@ variable {Symbol : Type _}
 
 /-- The language of an `Acceptor` is the set of strings it `Accepts`. -/
 @[scoped grind .]
-def language (a : Acceptor Symbol) : Language Symbol :=
-  { xs | a.Accepts xs }
+def language [Acceptor α Symbol] (a : α) : Language Symbol :=
+  { xs | Accepts a xs }
 
 /-- A string is in the language of an acceptor iff the acceptor accepts it. -/
 @[scoped grind =]
-theorem mem_language (a : Acceptor Symbol) (xs : List Symbol) :
-  xs ∈ a.language ↔ a.Accepts xs := Iff.rfl
+theorem mem_language [Acceptor α Symbol] (a : α) (xs : List Symbol) :
+  xs ∈ language a ↔ Accepts a xs := Iff.rfl
 
 end Acceptor
 
