Cslib/Computability/Automata/DAToNA.lean
@@ -4,10 +4,11 @@ Released under Apache 2.0 license as described in the file LICENSE.
 Authors: Fabrizio Montesi
 -/
 
-import Cslib.Computability.Automata.Deterministic.ExactAcceptor
-import Cslib.Computability.Automata.Nondeterministic.ExactAcceptor
+import Cslib.Computability.Automata.DA
+import Cslib.Computability.Automata.NA
+import Cslib.Foundations.Semantics.LTS.FLTSToLTS
 
-/-! # Translation of a `DA.ExactAcceptor` into an `NA.ExactAcceptor`.
+/-! # Translation of Deterministic Automata into Nonodeterministic Automata.
 
 This is the general version of the standard translation of DFAs into NFAs. -/
 
@@ -17,30 +18,25 @@ variable {State : Type _} {Symbol : Type _}
 
 section NA
 
--- /-- `DA` is a special case of `NA`. -/
--- @[scoped grind =]
--- def toNA (da : DA State Symbol) : NA State Symbol where
---   start := {da.start}
---   Tr := fun s1 μ s2 => da.tr s1 μ = s2
-
--- @[scoped grind =]
--- lemma toNA_start {da : DA State Symbol} : da.toNA.start = {da.start} := rfl
-
--- instance : Coe (DA State Symbol) (NA State Symbol) where
---   coe := toNA
-
-
-/-- The `NFA` constructed from a `DFA` has the same language. -/
+/-- `DA` is a special case of `NA`. -/
 @[scoped grind =]
-theorem toNA_exactAcceptor_language_eq {da : DA State Symbol} {acc : Set State} :
-    (da.exactAcceptor acc).language = (da.toNA.exactAcceptor acc).language := by
-  ext xs
-  apply Iff.intro <;> intro h
-  case mp =>
-    simp_all [NA.exactAcceptor, DA.exactAcceptor, Acceptor.language]
+def toNA (da : DA State Symbol) : NA State Symbol where
+  start := {da.start}
+  accept := da.accept
+  Tr := da.toLTS.Tr
 
-    open NA Acceptor DA in grind
-  refine ⟨?_, fun _ => ⟨da.start, ?_⟩⟩ <;> open NA Acceptor in grind
+instance : Coe (DA State Symbol) (NA State Symbol) where
+  coe := toNA
+
+/-- The `NA` constructed from a `DA` has the same language. -/
+@[scoped grind =]
+theorem toNA_language_eq {da : DA State Symbol} :
+    Acceptor.language da = Acceptor.language da.toNA := by
+  ext xs
+  refine ⟨?_, ?_⟩
+  · refine fun h => ⟨da.start, ?_⟩
+    open NA Acceptor FLTS in grind
+  · open NA Acceptor FLTS in grind
 
 end NA
 
