Cslib/Computability/Automata/NA.lean
@@ -10,11 +10,19 @@ import Cslib.Computability.Automata.Acceptor
 
 /-! # Nondeterministic Automaton
 
-A Nondeterministic Automaton (NA) is an automaton with a set of initial states.
+A Nondeterministic Automaton (NA) is a transition relation equipped with sets of initial and accept
+states.
 
 This definition extends `LTS` and thus stores the transition system as a relation `Tr` of the form
 `State → Symbol → State → Prop`. Note that you can also instantiate `Tr` by passing an argument of
 type `State → Symbol → Set State`; it gets automatically expanded to the former shape.
+
+This definition is a generalisation of NFAs found in the literature, without finiteness assumptions.
+
+## References
+
+* [J. E. Hopcroft, R. Motwani, J. D. Ullman,
+  *Introduction to Automata Theory, Languages, and Computation*][Hopcroft2006]
 -/
 
 namespace Cslib.Automata
@@ -25,16 +33,18 @@ structure NA (State : Type _) (Symbol : Type _) extends LTS State Symbol where
   /-- The set of accept states of the automaton. -/
   accept : Set State
 
-
 namespace NA
 
 variable {State : Type _} {Symbol : Type _}
 
 /-- An `NA` accepts a string if there is a multistep transition from a start state to an accept
-state. -/
+state.
+
+This is the standard string recognition performed by NFAs in the literature. -/
 @[scoped grind =]
-def acceptor (na : NA State Symbol) : Acceptor Symbol where
-  Accepts (xs : List Symbol) := ∃ s ∈ na.start, ∃ s' ∈ na.accept, na.MTr s xs s'
+instance : Acceptor (NA State Symbol) Symbol where
+  Accepts (na : NA State Symbol) (xs : List Symbol) :=
+    ∃ s ∈ na.start, ∃ s' ∈ na.accept, na.MTr s xs s'
 
 end NA
 
