Cslib/Computability/Automata/NAToDA.lean
@@ -4,11 +4,11 @@ Released under Apache 2.0 license as described in the file LICENSE.
 Authors: Fabrizio Montesi
 -/
 
-import Cslib.Computability.Automata.Deterministic.DA
-import Cslib.Computability.Automata.Nondeterministic.NA
+import Cslib.Computability.Automata.DA
+import Cslib.Computability.Automata.NA
 import Cslib.Foundations.Semantics.LTS.LTSToFLTS
 
-/-! # Translation of NFA into DFA (subset construction) -/
+/-! # Translation of Nondeterministic Automata into Deterministic Automata (subset construction) -/
 
 namespace Cslib.Automata.NA
 
@@ -27,18 +27,14 @@ def toDA (na : NA State Symbol) : DA (Set State) Symbol := {
 /-- The `DA` constructed from an `NA` has the same language. -/
 @[scoped grind =]
 theorem toDA_language_eq {na : NA State Symbol} :
-  na.toDA.acceptor.language = na.acceptor.language := by
+  Acceptor.language na.toDA = Acceptor.language na := by
   ext xs
-  -- simp [toDA, NA.acceptor, DA.acceptor]
-  rw [Acceptor.mem_language]
-  rw [Acceptor.mem_language]
-  -- simp [LTS.toFLTS]
   #adaptation_note
   /--
   Moving from `nightly-2025-09-15` to `nightly-2025-10-19` required
   increasing the number of allowed splits.
   -/
-  open DA NA Acceptor FLTS LTS in grind (splits := 12)
+  open DA Acceptor LTS in grind (splits := 11)
 
 end SubsetConstruction
 
