Cslib/Foundations/Semantics/LTS/FLTSToLTS.lean
@@ -21,7 +21,7 @@ instance : Coe (FLTS State Label) (LTS State Label) where
 
 /-- `FLTS.toLTS` correctly characterises transitions. -/
 @[scoped grind =]
-theorem toLTS_tr {flts : FLTS State Label} {s1 s2 : State} {μ : Label} :
+theorem toLTS_tr {flts : FLTS State Label} {s1 : State} {μ : Label} {s2 : State} :
   flts.toLTS.Tr s1 μ s2 ↔ flts.tr s1 μ = s2 := by rfl
 
 /-- The transition system of a FLTS is deterministic. -/
@@ -36,7 +36,7 @@ theorem toLTS_imageFinite (flts : FLTS State Label) : flts.toLTS.ImageFinite :=
 
 /-- Characterisation of multistep transitions. -/
 @[scoped grind =]
-theorem toLTS_mtr {flts : FLTS State Label} {s1 s2 : State} {μs : List Label} :
+theorem toLTS_mtr {flts : FLTS State Label} {s1 : State} {μs : List Label} {s2 : State} :
     flts.toLTS.MTr s1 μs s2 ↔ flts.mtr s1 μs = s2 := by
   have : ∀ μ, flts.toLTS.Tr s1 μ (flts.tr s1 μ) := by grind
   constructor <;> intro h
